WIP: Add pairs of words as a kind of value
64-bit pairs of 32-bit words allow us to model the values stored in the
individual parts of register pairs. A pair may be partial: only the high or
the low part might be defined. This is reflected in the constructors. If
both parts are undefined, we simply have an undefined value.

cfrontend/PrintCsyntax.ml
@@ -190,6 +190,8 @@ let print_typed_value p v ty =
       fprintf p "<ptr%a>" !print_pointer_hook (b, ofs)
   | Vundef, _ ->
       fprintf p "<undef>"
+  | Vpair _, _ ->
+      fprintf p "<pair>"
 
 let print_value p v = print_typed_value p v Tvoid
 
